thys/Registers/Axioms_Complement.thy
@@ -1,21 +1,40 @@
 section \<open>Axioms of complements\<close>
 
 theory Axioms_Complement
-  imports Laws
+  imports Laws With_Type.With_Type
+(* With_Type.With_Type_Inst_HOL *)
 begin
 
 typedecl ('a, 'b) complement_domain
 instance complement_domain :: (domain, domain) domain..
+typedecl ('a, 'b) complement_domain_simple
+instance complement_domain_simple :: (domain, domain) domain..
+
+setup \<open> (* Supporting with-type for the dummy class `domain` *)
+With_Type.add_with_type_info_global {
+  class = \<^class>\<open>domain\<close>,
+  rep_class_data = \<^const_name>\<open>with_type_type_class\<close>,
+  with_type_compat_rel = @{thm with_type_compat_rel_type},
+  rep_class_data_thm = NONE,
+  transfer = NONE
+}\<close>
 
 \<comment> \<open>We need that there is at least one object in our category. We call is \<^term>\<open>some_domain\<close>.\<close>
 typedecl some_domain
 instance some_domain :: domain..
 
-class simple_complement_domain = domain
+class domain_with_simple_complement = domain
 
 axiomatization where 
   complement_exists_simple: \<open>register F \<Longrightarrow> \<exists>G :: ('a, 'b) complement_domain update \<Rightarrow> 'b update. compatible F G \<and> iso_register (F;G)\<close>
-    for F :: \<open>'a::domain update \<Rightarrow> 'b::simple_complement_domain update\<close>
+    for F :: \<open>'a::domain update \<Rightarrow> 'b::domain_with_simple_complement update\<close>
+
+term \<open>\<forall>\<^sub>\<tau> 'c::domain = register_decomposition_domain F. xxx\<close>
+
+axiomatization complement_domain :: \<open>('a::domain update \<Rightarrow> 'b::domain update) \<Rightarrow> ('a,'b) complement_domain set\<close> where 
+  complement_exists: \<open>register F \<Longrightarrow> \<forall>\<^sub>\<tau> 'c::domain = complement_domain F.
+                      \<exists>G :: 'c update \<Rightarrow> 'b update. compatible F G \<and> iso_register (F;G)\<close>
+    for F :: \<open>'a::domain update \<Rightarrow> 'b::domain update\<close>
 
 axiomatization where complement_unique: \<open>compatible F G \<Longrightarrow> iso_register (F;G) \<Longrightarrow> compatible F H \<Longrightarrow> iso_register (F;H)
           \<Longrightarrow> equivalent_registers G H\<close> 
